Pdec <= Pinst proof done! But need to optimize the proof

examples/ProcDecInv.v
@@ -4,7 +4,7 @@ Require Import Lib.Struct Lib.StringBound Lib.FMap Lib.StringEq.
 Require Import Lts.Syntax Lts.Semantics Lts.Equiv Lts.Refinement Lts.Renaming Lts.Wf.
 Require Import Lts.Renaming Lts.Specialize Lts.Inline Lts.InlineFacts_2 Lts.DecompositionZero.
 Require Import Ex.SC Ex.Fifo Ex.MemAtomic Ex.ProcDec Ex.ProcDecInl.
-Require Import Eqdep.
+Require Import Eqdep ProofIrrelevance.
 
 Set Implicit Arguments.
 
@@ -53,35 +53,74 @@ Ltac simpl_find :=
 Ltac invReify :=
   repeat (eexists; split; [findReify; simpl; eauto|]).
 
+Ltac inv_contra :=
+  try (exfalso; repeat autounfold with InvDefs in *; dest; subst;
+       repeat
+         (match goal with
+          | [H: false = true |- _] => inversion H
+          | [H: true = false |- _] => inversion H
+          | [H: negb _ = true |- _] => apply negb_true_iff in H; subst
+          | [H: negb _ = false |- _] => apply negb_false_iff in H; subst
+          end; dest; try subst);
+       fail).
+
 Ltac inv_red :=
-  repeat autounfold with InvDefs in *; dest; simpl_find;
+  repeat autounfold with InvDefs in *; dest;
   repeat
     (match goal with
-     (* Logic *)
      | [ |- ~ _ ] => intro
-     | [H: _ \/ _ |- _] => destruct H
-     | [ |- _ /\ _ ] => split
      | [H: ?t = ?t |- _] => clear H
-     (* Reducing boolean conditions *)
-     | [H: false = true |- _] => inversion H
-     | [H: true = false |- _] => inversion H
      | [H: negb _ = true |- _] => apply negb_true_iff in H; subst
      | [H: negb _ = false |- _] => apply negb_false_iff in H; subst
      end; dest; try subst).
 
+Lemma rewrite_not_weq: forall sz (a b: word sz) (pf: a <> b), weq a b = right _ pf.
+Proof.
+  intros; destruct (weq a b); try solve [ elimtype False; auto ].
+  f_equal; apply proof_irrelevance.
+Qed.
+
 Ltac inv_solve :=
-  abstract (
-      inv_red;
-      repeat
-        (try
-           match goal with
-           (* Destruction *)
-           | [H: context [weq ?w1 ?w2] |- _] => destruct (weq w1 w2)
-           | [ |- context [weq ?w1 ?w2] ] => destruct (weq w1 w2)
-           end;
-         try subst;
-         intuition idtac)
-    ).
+  repeat
+    (inv_red;
+     repeat
+       match goal with
+       | [ |- _ /\ _ ] => split
+       (* For optimized destruction of "weq" *)
+       | [ |- context[weq ?w ?w] ] =>
+         let H := fresh "H" in
+         pose proof (@rewrite_weq _ w w eq_refl) as H; rewrite H; clear H
+       | [ |- context[weq ?w1 ?w2] ] =>
+         let H := fresh "H" in
+         let Hr := fresh "Hr" in
+         assert (w1 = w2) as H by reflexivity;
+         pose proof (@rewrite_weq _ w1 w2 H) as Hr;
+         rewrite Hr; clear Hr H
+       | [ |- context[weq ?w1 ?w2] ] =>
+         let H := fresh "H" in
+         let Hr := fresh "Hr" in
+         assert (w1 <> w2) as H by discriminate;
+         pose proof (@rewrite_not_weq _ w1 w2 H) as Hr;
+         rewrite Hr; clear Hr H
+       (* Normal destruction of "weq": it's slow *)
+       | [H: context [weq ?w1 ?w2] |- _] => destruct (weq w1 w2)
+       | [ |- context [weq ?w1 ?w2] ] => destruct (weq w1 w2)
+       | [ |- context [weq ?w ?w] ] =>
+         let n := fresh "n" in
+         destruct (weq w w) as [|n]; [|elim n; reflexivity]
+       end;
+     try subst;
+     inv_contra;
+     intuition auto).
+
+Definition or3 (b1 b2 b3: Prop) := b1 \/ b2 \/ b3.
+Tactic Notation "or3_fst" := left.
+Tactic Notation "or3_snd" := right; left.
+Tactic Notation "or3_thd" := right; right.
+Ltac dest_or3 :=
+  match goal with
+  | [H: or3 _ _ _ |- _] => destruct H as [|[|]]
+  end.
 
 Section Invariants.
   Variables addrSize fifoSize valSize rfIdx: nat.
@@ -109,49 +148,48 @@ Section Invariants.
     exact True.
   Defined.
 
-  Definition xor3 (b1 b2 b3: Prop) :=
-    (b1 /\ (~ b2) /\ (~ b3)) \/
-    ((~ b1) /\ b2 /\ (~ b3)) \/
-    ((~ b1) /\ (~ b2) /\ b3).
-
   Definition fifo_empty_inv (fifoEmpty: bool) (fifoEnqP fifoDeqP: type (Bit fifoSize)): Prop :=
     fifoEmpty = true /\ fifoEnqP = fifoDeqP.
   
   Definition fifo_not_empty_inv (fifoEmpty: bool) (fifoEnqP fifoDeqP: type (Bit fifoSize)): Prop :=
     fifoEmpty = false /\ fifoEnqP = fifoDeqP ^+ $1.
 
-  Hint Unfold xor3 fifo_empty_inv fifo_not_empty_inv: InvDefs.
+  Definition mem_request_inv
+             (pc: fullType type (SyntaxKind (Bit addrSize)))
+             (rf: fullType type (SyntaxKind (Vector (Bit valSize) rfIdx)))
+             (insEmpty: bool) (insElt: type (Vector (memAtomK addrSize valSize) fifoSize))
+             (insDeqP: type (Bit fifoSize)): Prop.
+  Proof.
+    refine (if insEmpty then True else _).
+    refine (_ /\ _ /\ _).
+    - exact (insElt insDeqP ``"type" = dec _ rf pc ``"opcode").
+    - exact (insElt insDeqP ``"addr" = dec _ rf pc ``"addr").
+    - refine (if weq (insElt insDeqP ``"type") (evalConstT memLd) then _ else _).
+      + exact (insElt insDeqP ``"value" = evalConstT (getDefaultConst (Bit valSize))).
+      + refine (if weq (insElt insDeqP ``"type") (evalConstT memSt) then _ else True).
+        exact (insElt insDeqP ``"value" = dec _ rf pc ``"value").
+  Defined.
+
+  Hint Unfold fifo_empty_inv fifo_not_empty_inv mem_request_inv: InvDefs.
 
   Definition procDec_inv_1 (o: RegsT): Prop.
   Proof.
+    kexistv "pc"%string pcv o (Bit addrSize).
+    kexistv "rf"%string rfv o (Vector (Bit valSize) rfIdx).
     kexistv "stall"%string stallv o Bool.
     kexistv "Ins.empty"%string iev o Bool.
     kexistv "Ins.enqP"%string ienqP o (Bit fifoSize).
     kexistv "Ins.deqP"%string ideqP o (Bit fifoSize).
+    kexistv "Ins.elt"%string ieltv o (Vector (memAtomK addrSize valSize) fifoSize).
     kexistv "Outs.empty"%string oev o Bool.
     kexistv "Outs.enqP"%string oenqP o (Bit fifoSize).
     kexistv "Outs.deqP"%string odeqP o (Bit fifoSize).
-    refine (xor3 _ _ _).
-    - exact (v = false /\ fifo_empty_inv v0 v1 v2 /\ fifo_empty_inv v3 v4 v5).
-    - exact (v = true /\ fifo_not_empty_inv v0 v1 v2 /\ fifo_empty_inv v3 v4 v5).
-    - exact (v = true /\ fifo_empty_inv v0 v1 v2 /\ fifo_not_empty_inv v3 v4 v5).
-  Defined.
-
-  Definition procDec_inv_2 (o: RegsT): Prop.
-  Proof.
-    kexistv "pc"%string pcv o (Bit addrSize).
-    kexistv "rf"%string rfv o (Vector (Bit valSize) rfIdx).
-    kexistv "Ins.empty"%string iev o Bool.
-    kexistv "Ins.elt"%string ieltv o (Vector (memAtomK addrSize valSize) fifoSize).
-    kexistv "Ins.deqP"%string ideqP o (Bit fifoSize).
-    refine (if v1 then True else _).
-    refine (_ /\ _ /\ _).
-    - exact (v2 v3 ``"type" = dec _ v0 v ``"opcode").
-    - exact (v2 v3 ``"addr" = dec _ v0 v ``"addr").
-    - refine (if weq (v2 v3 ``"type") (evalConstT memLd) then _ else _).
-      + exact (v2 v3 ``"value" = evalConstT (getDefaultConst (Bit valSize))).
-      + refine (if weq (v2 v3 ``"type") (evalConstT memSt) then _ else True).
-        exact (v2 v3 ``"value" = dec _ v0 v ``"value").
+    refine (or3 _ _ _).
+    - exact (v1 = false /\ fifo_empty_inv v2 v3 v4 /\ fifo_empty_inv v6 v7 v8).
+    - refine (_ /\ _).
+      + exact (v1 = true /\ fifo_not_empty_inv v2 v3 v4 /\ fifo_empty_inv v6 v7 v8).
+      + exact (mem_request_inv v v0 v2 v5 v4).
+    - exact (v1 = true /\ fifo_empty_inv v2 v3 v4 /\ fifo_not_empty_inv v6 v7 v8).
   Defined.
 
   Lemma procDec_inv_0_ok':
@@ -220,7 +258,7 @@ Section Invariants.
     (* - repeat subst. *)
     (*   simpl; unfold procDec_inv_1. *)
     (*   invReify. *)
-    (*   left; inv_solve. *)
+    (*   or3_fst; inv_solve. *)
 
     (* - specialize (IHMultistep H); clear -IHMultistep HStep. *)
     (*   apply step_no_defs_substep in HStep; [|reflexivity]. *)
@@ -231,33 +269,58 @@ Section Invariants.
     (*   + inv H; invertActionRep. *)
     (*     unfold procDec_inv_1 in *; dest. *)
     (*     invReify; simpl_find. *)
-    (*     right; left; repeat split; inv_solve. *)
+        
+    (*     dest_or3; inv_contra. *)
+    (*     or3_snd; repeat split; inv_solve. *)
+
     (*   + inv H0; invertActionRep. *)
     (*     unfold procDec_inv_1 in *; dest. *)
     (*     invReify; simpl_find. *)
-    (*     right; left; repeat split; inv_solve. *)
+
+    (*     dest_or3; inv_contra. *)
+    (*     or3_snd; repeat split; inv_solve. *)
+        
     (*   + inv H; invertActionRep. *)
     (*     unfold procDec_inv_1 in *; dest. *)
     (*     invReify; simpl_find. *)
-    (*     left; repeat split; inv_solve. *)
+
+    (*     dest_or3; inv_contra. *)
+    (*     or3_fst; repeat split; inv_solve. *)
+        
     (*   + inv H0; invertActionRep. *)
     (*     unfold procDec_inv_1 in *; dest. *)
     (*     invReify; simpl_find. *)
-    (*     left; repeat split; inv_solve. *)
+
+    (*     dest_or3; inv_contra. *)
+    (*     or3_fst; repeat split; inv_solve. *)
+        
     (*   + inv H; invertActionRep. *)
     (*     unfold procDec_inv_1 in *; dest. *)
-    (*     invReify; simpl_find; auto. *)
+    (*     invReify; simpl_find. *)
+
+    (*     dest_or3; inv_contra. *)
+    (*     or3_fst; repeat split; inv_solve. *)
+        
     (*   + inv H0; invertActionRep. *)
     (*     unfold procDec_inv_1 in *; dest. *)
-    (*     invReify; simpl_find; auto. *)
+    (*     invReify; simpl_find. *)
+
+    (*     dest_or3; inv_contra. *)
+    (*     or3_fst; repeat split; inv_solve. *)
+
     (*   + inv H; invertActionRep. *)
     (*     unfold procDec_inv_1 in *; dest. *)
     (*     invReify; simpl_find. *)
-    (*     right; right; repeat split; inv_solve. *)
+
+    (*     dest_or3; inv_contra. *)
+    (*     or3_thd; repeat split; inv_solve. *)
+
     (*   + inv H0; invertActionRep. *)
     (*     unfold procDec_inv_1 in *; dest. *)
     (*     invReify; simpl_find. *)
-    (*     right; right; repeat split; inv_solve. *)
+
+    (*     dest_or3; inv_contra. *)
+    (*     or3_thd; repeat split; inv_solve. *)
   Qed.
 
   Lemma procDec_inv_1_ok:
@@ -269,26 +332,8 @@ Section Invariants.
     eapply procDec_inv_1_ok'; eauto.
   Qed.
 
-  Lemma procDec_inv_2_ok':
-    forall init n ll,
-      init = initRegs (getRegInits (fst pdecInl)) ->
-      Multistep (fst pdecInl) init n ll ->
-      procDec_inv_2 n.
-  Proof.
-    admit.
-  Qed.
-
-  Lemma procDec_inv_2_ok:
-    forall o,
-      reachable o (fst pdecInl) ->
-      procDec_inv_2 o.
-  Proof.
-    intros; inv H; inv H0.
-    eapply procDec_inv_2_ok'; eauto.
-  Qed.
-
 End Invariants.
 
-Hint Unfold xor3 procDec_inv_0 procDec_inv_1 procDec_inv_2
-     fifo_empty_inv fifo_not_empty_inv: InvDefs.
+Hint Unfold procDec_inv_0 procDec_inv_1
+     fifo_empty_inv fifo_not_empty_inv mem_request_inv: InvDefs.
 
